@@ -33,7 +33,7 @@ def ktSlots : Nat := kvFrameSlots - 32
 def wp_kerneltrap_body {hlc : HasLC} {GF : BundledGFunctors} [MachGS hlc GF] [Xv6G GF] [CurCtx]
     (cpu : CPU) (k : KCtx) (epc sc : BitVec 64)
     (hsie : k.sie = false) (hspie : k.spie = true) (hspp : k.spp = true)
-    (hnoff : k.noff = 0) (hlocks : k.locks = []) (hK : ktSlots ≤ k.avail)
+    (hnoff : k.noff = 0) (hlocks : k.locks = []) (htier : k.tier = KTier.kpt) (hK : ktSlots ≤ k.avail)
     (hsc : sCauseOk sc) (hepc : epc.toNat % 2 = 0) : Prop :=
   kctx cpu k ∗ pcIs cpu kerneltrapAddr ∗ trapCsrsAt cpu epc sc 0#64 ∗ cpuClaim k.proc ∗ intrRes cpu ∗
   wpNext true k.proc cpu (fun cpu' => iprop(∀ (R' : RegMap) (sc' tv' : BitVec 64),
@@ -44,7 +44,7 @@ def wp_kerneltrap_body {hlc : HasLC} {GF : BundledGFunctors} [MachGS hlc GF] [Xv
 /-- The interface of `kerneltrap`. -/
 structure KERNELTRAP : Prop where
   wp_kerneltrap : ∀ {hlc : HasLC} {GF : BundledGFunctors} [MachGS hlc GF] [Xv6G GF] [CurCtx]
-    (cpu : CPU) (k : KCtx) (epc sc : BitVec 64) hsie hspie hspp hnoff hlocks hK hsc hepc,
-    wp_kerneltrap_body (hlc := hlc) (GF := GF) cpu k epc sc hsie hspie hspp hnoff hlocks hK hsc hepc
+    (cpu : CPU) (k : KCtx) (epc sc : BitVec 64) hsie hspie hspp hnoff hlocks htier hK hsc hepc,
+    wp_kerneltrap_body (hlc := hlc) (GF := GF) cpu k epc sc hsie hspie hspp hnoff hlocks htier hK hsc hepc
 
 end Xv6
